coq/Integers.v
@@ -1,0 +1,24 @@
+From Vellvm Require Import
+     Numeric.Integers.
+
+Class FInt I : Type :=
+  { add  : I -> I -> I;
+    sub  : I -> I -> I;
+    mul  : I -> I -> I;
+    eq   : I -> I -> bool;
+    zero : I;
+  }.
+
+Instance FInt64 : FInt Int64.int :=
+  {| add  := Int64.add;
+     sub  := Int64.sub;
+     mul  := Int64.mul;
+     eq   := Int64.eq;
+     zero := Int64.zero;
+  |}.
+
+Inductive PrimOp : Set :=
+| Mul
+| Add
+| Sub
+.
