coq/TestUtils.v
@@ -1,0 +1,35 @@
+From Coq Require Import
+     String.
+
+From QuickChick Require Import QuickChick.
+
+From ITree Require Import
+     ITree
+     Interp.Recursion
+     Events.Exception.
+
+Require Import SystemF.
+
+Inductive MlResult a e :=
+| MlOk : a -> MlResult a e
+| MlError : e -> MlResult a e.
+
+Extract Inductive MlResult => "result" [ "Ok" "Error" ].
+
+Unset Guard Checking.
+Fixpoint run_eval (t : ITreeDefinition.itree Failure Term) : MlResult Term string
+  := match observe t with
+     | RetF x => MlOk _ string x
+     | TauF t => run_eval t
+     | VisF _ (Throw msg) k => MlError _ string msg
+     end.
+Set Guard Checking.
+
+Instance showMLResult {A E} `{Show A} `{Show E} : Show (MlResult A E)
+  := {| show :=
+          fun mlr =>
+            match mlr with
+            | MlOk x => "MlOk " ++ show x
+            | MlError x => "MlError " ++ show x
+            end
+    |}.
